before proof of forward simulation (injp_C @ CA)

demo/DemoBproofnew.v
@@ -14,114 +14,20 @@ Require Import CallConv Compiler CA.
 
 Require Import CKLRAlgebra Extends Inject InjectFootprint.
 
+(* forget it for now
 Search wt_c.
+*)
 
-Module C_injp.
+Section injp_CA.
 
-Inductive state: Type :=
-| Callstateg
-    (ai: int)
-    (m: mem)
-| Callstatef
-    (sp: val)
-    (aif: int)
-    (m: mem)
-| Returnstatef
-    (sp: val)
-    (aif: int)
-    (rig: int)
-    (m: mem)
-| Returnstateg
-    (ri: int)
-    (m: mem).
+Lemma injp_CA: forward_simulation
+                 (cc_c injp @ cc_c_asm)
+                 (cc_c injp @ cc_c_asm)
+                 Bspec (Asm.semantics prog).
+Proof.
+ Admitted.
 
-Section WITH_SE.
-  Context (se: Genv.symtbl).
-
-Inductive initial_state : query li_c -> state -> Prop :=
-| initial_state_intro
-    v args m b i
-    (SYMB: Genv.symbol_address se g_id Ptrofs.zero = v)
-    (FPTR: v = Vptr b Ptrofs.zero)
-(*    (RANGE: 0 <= i.(Int.intval) < MAX) *)
-    (VS: args = (Vint i:: nil)):
-    initial_state (cq v int_int_sg ((Vint i) :: nil) m) (Callstateg i m).
-
-Inductive at_external: state -> query li_c -> Prop :=
-| at_external_intro
-    g_fptr aif m sp
-    (VALID: valid_blockv (Mem.support m) sp)
-    (FINDG: Genv.symbol_address se f_id Ptrofs.zero = Vptr g_fptr Ptrofs.zero):
-    at_external (Callstatef sp aif m)
-                (cq (Vptr g_fptr Ptrofs.zero) int_int_sg ((Vint (Int.sub aif Int.one)) :: nil) m).
-
-Inductive after_external: state -> reply li_c -> state -> Prop :=
-| after_external_intro
-    aif ti m m' sp
-    (UNCHANGE: Mem.unchanged_on (fun b _  => sp = Vptr b Ptrofs.zero) m m'):
-    after_external (Callstatef sp aif m) (cr (Vint ti) m') (Returnstatef sp aif ti m').
-
-Inductive step : state -> trace -> state -> Prop :=
-| step_zero
-    i m
-    (ZERO: i.(Int.intval) = 0%Z):
-    step (Callstateg i m) E0 (Returnstateg (Int.zero) m)
-| step_read
-    i b_mem m ti
-    (NZERO: i.(Int.intval) <> 0%Z)
-    (FINDM: Genv.symbol_address se _memoized (Ptrofs.repr 4) = Vptr b_mem (Ptrofs.repr 4))
-    (LOAD1: Mem.loadv Mint32 m (Vptr b_mem (Ptrofs.repr 4)) = Some (Vint ti)):
-      step (Callstateg i m) E0 (Returnstateg ti m)
-| step_call
-    i m i' b_mem m' sb
-    (NZERO: i.(Int.intval) <> 0%Z)
-    (FINDM: Genv.symbol_address se _memoized Ptrofs.zero= Vptr b_mem Ptrofs.zero)
-    (LOAD0: Mem.loadv Mint32 m (Vptr b_mem Ptrofs.zero) = Some (Vint i'))
-    (NEQ: i <> i')
-    (ALLOC: Mem.alloc m 0 24 = (m',sb)):
-    step (Callstateg i m) E0 (Callstatef (Vptr sb Ptrofs.zero) i m')
-| step_return
-    b_mem m m' m'' ti i
-    (FINDM: Genv.symbol_address se _memoized Ptrofs.zero  = Vptr b_mem Ptrofs.zero)
-    (STORE0: Mem.storev Mint32 m (Vptr b_mem Ptrofs.zero) (Vint i) = Some m')
-    (STORE0: Mem.storev Mint32 m' (Vptr b_mem (Ptrofs.repr 4)) (Vint (Int.add ti i)) = Some m''):
-    step (Returnstatef i ti m) E0 (Returnstateg (Int.add ti i) m'').
-
-Inductive final_state: state -> reply li_c  -> Prop :=
-  | final_state_intro
-      s m:
-      final_state (Returnstateg s m) (cr (Vint s) m).
-
-End WITH_SE.
-
-Program Definition Bspec : Smallstep.semantics li_c li_c :=
-  {|
-   Smallstep.skel := erase_program DemoB.prog;
-   Smallstep.state := state;
-   Smallstep.activate se :=
-     let ge := Genv.globalenv se DemoB.prog in
-     {|
-       Smallstep.step ge := step ge;
-       Smallstep.valid_query q := Genv.is_internal ge (cq_vf q);
-       Smallstep.initial_state := initial_state ge;
-       Smallstep.at_external := at_external ge;
-       Smallstep.after_external := after_external;
-       Smallstep.final_state := final_state;
-       globalenv := ge;
-     |}
-   |}.
-
-End C_injp.
-Variable Bspec' : Smallstep.semantics li_c li_c.
-
-Axiom injp_protection : forward_simulation
-                          (cc_c injp) (cc_c injp) Bspec Bspec'.
-
-Variable self_wt : forward_simulation (wt_c @ lessdef_c) (wt_c @ lessdef_c) Bspec' Bspec'.
-
-Axiom CA : forward_simulation (cc_c_asm) (cc_c_asm) Bspec' (Asm.semantics DemoB.prog).
-
-
+(*
 Theorem Bproof :
   forward_simulation cc_compcert cc_compcert Bspec (Asm.semantics DemoB.prog).
 Proof.
@@ -141,3 +47,4 @@ Proof.
   eapply CA.
   eapply semantics_asm_rel; eauto.
 Qed.
+*)
